new approach about substs...

co_kind.v
@@ -3,98 +3,117 @@ Require Import LibTactics.
 Require Import Program.Wf.
 Require Import Arith.
 
-Require Import coercion subst type tactics.
+Require Import coercion type tactics ty_kind subst.
+
+Reserved Notation "Si |-co g ~: t1 ~~ t2" (at level 67, t1 at next level).
+Inductive co_kind : ctxt -> coercion -> type -> type -> Prop :=
+| CKRefl : forall Si t k,
+             Si |-ty t ~: k ->
+             Si |-co CRefl t ~: t ~~ t
+| CKSym : forall Si g t1 t2,
+            Si |-co g ~: t1 ~~ t2 ->
+            Si |-co CSym g ~: t2 ~~ t1
+| CKTrans : forall Si g1 g2 t1 t2 t3,
+              Si |-co g1 ~: t1 ~~ t2 ->
+              Si |-co g2 ~: t2 ~~ t3 ->
+              Si |-co CTrans g1 g2 ~: t1 ~~ t3
+| CKArrow : forall Si g1 g2 t1 t1' t2 t2',
+              Si |-co g1 ~: t1 ~~ t2 ->
+              Si |-co g2 ~: t1' ~~ t2' ->
+              Si |-co CArrow g1 g2 ~: TArrow t1 t1' ~~ TArrow t2 t2'
+| CKApp : forall Si g1 g2 t1 t1' t2 t2',
+            Si |-co g1 ~: t1 ~~ t2 ->
+            Si |-co g2 ~: t1' ~~ t2' ->
+            Si |-co CApp g1 g2 ~: TApp t1 t1' ~~ TApp t2 t2'
+| CKLeft : forall Si g t1 t1' t2 t2',
+             Si |-co g ~: TApp t1 t1' ~~ TApp t2 t2' ->
+             Si |-co CLeft g ~: t1 ~~ t2
+| CKRight : forall Si g t1 t1' t2 t2',
+              Si |-co g ~: TApp t1 t1' ~~ TApp t2 t2' ->
+              Si |-co CRight g ~: t1' ~~ t2'
+| CKFun : forall Si g t1 t2 f,
+            Si |-co g ~: t1 ~~ t2 ->
+            Si |-co CFun f g ~: TFun f t1 ~~ TFun f t2
+| CKAx : forall ax ks f typat rhs axs funs tcs tys,
+           ok_ctxt (funs, axs, tcs) -> 
+           binds ax (mkAxiom ks f typat rhs) axs ->
+           (funs, axs, tcs)|-co CAx ax tys ~: TFun f (typat [^tys]) ~~ (rhs[^tys])
+where "Si |-co g ~: t1 ~~ t2" := (co_kind Si g t1 t2).
 
 Parameter ok__unique : forall {A} x (v v' : A) E,
   ok E -> binds x v E -> binds x v' E -> v = v'.
 
-Axiom notin_subset : forall (x : var) L L',
-  x \notin L' -> L \c L' -> x \notin L.
-
-Lemma ty_kind_reg : forall Si D t k,
-  Si; D |-ty t ~: k ->
-  ok_gr Si /\ ok D.
+Lemma ty_kind_reg : forall Si t k,
+  Si |-ty t ~: k ->
+  ok_ctxt Si.
 Proof.
   induction 1; try tauto.
-  pick_fresh_gen L x. specialize (H0 x). apply H0 in Fr. intuition.
 Qed.
 
-Lemma co_kind_reg : forall Si D co t1 t2,
-  Si; D |-co co ~: t1 ~~ t2 ->
-  ok_gr Si /\ ok D.
+Lemma co_kind_reg : forall Si co t1 t2,
+  Si |-co co ~: t1 ~~ t2 ->
+  ok_ctxt Si.
 Proof.
   induction 1; auto.
   eapply ty_kind_reg. eassumption.
-  pick_fresh_gen L x. specialize (H1 x). apply H1 in Fr. intuition.
 Qed.
 
-Lemma size_of_ty_open : forall ty n x,
-  size_of_ty ty = size_of_ty ({n ~> TFVar (v x)}ty).
-Proof.
-  induction ty; intros; simpl; try omega; auto.
-  destruct (eq_nat_decide n0 n); simpl; auto.
-Qed.
-
-Lemma size_of_co_open : forall co n x,
-  size_of_co co = size_of_co ({n ~> TFVar (v x)}co).
-Proof.
-  induction co; intros; simpl; try omega; auto.
-  f_equal. apply size_of_ty_open.
-  f_equal. induction l; simpl. reflexivity. rewrite <- size_of_ty_open. rewrite <- IHl.
-    reflexivity.
-Qed.
-
-Lemma co_kind_det : forall Si D co t1 t2,
-  Si; D |-co co ~: t1 ~~ t2 ->
+Lemma co_kind_det : forall Si co t1 t2,
+  Si|-co co ~: t1 ~~ t2 ->
   forall t3 t4,
-  Si; D |-co co ~: t3 ~~ t4 ->
+  Si|-co co ~: t3 ~~ t4 ->
   t1 = t3 /\ t2 = t4.
 Proof.
-  induction 1; inversion 1; subst; auto.
-  - apply IHco_kind in H4. tauto.
-  - apply IHco_kind1 in H6. apply IHco_kind2 in H9. tauto.
-  - apply IHco_kind1 in H6. apply IHco_kind2 in H9. intuition; subst; auto.
-  - pick_fresh_gen (L0 \u L) x. specialize (H10 x). lapplies H10; auto.
-    specialize (H1 x). lapplies H1; auto. apply H4 in H3. intuition; f_equal; auto.
-  - apply IHco_kind1 in H6. apply IHco_kind2 in H9. intuition; subst; auto.
-  - apply IHco_kind in H4. inverts H4. inverts H1. inverts H2. auto.
-  - apply IHco_kind in H4. inverts H4. inverts H1. inverts H2. auto.
-  - apply IHco_kind in H7. intuition; subst; auto.
-  - pose proof (ok__unique ax (mkAxiom ks f typat rhs)
-                                     (mkAxiom ks0 f0 typat0 rhs0) axs). lapplies H3; auto.
-    inverts H4. auto. unfolds ok_gr. tauto. 
+  Ltac co_kind_det :=
+    repeat match goal with
+      | [ IH : forall _ _, _ |-co ?g ~: _ ~~ _ -> _,
+            H : _ |-co ?g ~: _ ~~ _
+            |- _ ] => apply IH in H
+    end;
+    repeat match goal with
+             | [ H : _ = _ /\ _ = _ |- _ ] => inverts H
+             | [ H : TApp _ _ = TApp _ _ |- _ ] => inverts H
+             | [ H : TArrow _ _ = TArrow _ _ |- _ ] => inverts H
+           end.
+
+  induction 1; inversion 1; auto; co_kind_det; auto.
+  match goal with
+    | [ H1 : binds ?ax (mkAxiom ?ks1 ?f1 ?typat1 ?rhs1) _
+      , H2 : binds ?ax (mkAxiom ?ks2 ?f2 ?typat2 ?rhs2) _
+        |- TFun ?f1 (?typat1 [^_]) = TFun ?f2 (?typat2 [^_]) /\
+           ?rhs1[^_] = ?rhs2[^_] ] =>
+      pose proof (ok__unique ax (mkAxiom ks1 f1 typat1 rhs1)
+                                (mkAxiom ks2 f2 typat2 rhs2) axs) as Hunique
+  end. lapplies Hunique. inverts H11. auto. auto. auto. inverts H. tauto.
 Qed.
- 
-Program Fixpoint coercionKind funs axs tcs D co 
-        (_ : exists t1 t2, (funs,axs,tcs); D |-co co ~: t1 ~~ t2) 
-        { measure (size_of_co co) } :
-  sig ( fun types : (type * type) =>
-          (funs, axs, tcs); D |-co co ~: (fst types) ~~ (snd types) ) :=
+
+Unset Transparent Obligations.
+Program Fixpoint coercionKind funs axs tcs co 
+        (_ : exists t1 t2, (funs,axs,tcs)|-co co ~: t1 ~~ t2) 
+        { measure (size_of_co false co) } :
+  { types : (type * type) |
+          (funs, axs, tcs)|-co co ~: (fst types) ~~ (snd types) } :=
   match co with
     | CRefl ty => (ty, ty)
-    | CSym co => let types := coercionKind funs axs tcs D co _ in (snd types, fst types)
-    | CTrans co1 co2 => let tys1 := coercionKind funs axs tcs D co1 _ in
-                        let tys2 := coercionKind funs axs tcs D co2 _ in
+    | CSym co => let types := coercionKind funs axs tcs co _ in (snd types, fst types)
+    | CTrans co1 co2 => let tys1 := coercionKind funs axs tcs co1 _ in
+                        let tys2 := coercionKind funs axs tcs co2 _ in
                         (fst tys1, snd tys2)
-    | CArrow co1 co2 => let tys1 := coercionKind funs axs tcs D co1 _ in
-                        let tys2 := coercionKind funs axs tcs D co2 _ in
+    | CArrow co1 co2 => let tys1 := coercionKind funs axs tcs co1 _ in
+                        let tys2 := coercionKind funs axs tcs co2 _ in
                         (TArrow (fst tys1) (fst tys2), TArrow (snd tys1) (snd tys2))
-    | CForAll ki co => let x := var_gen (dom D) in
-                       let tys := coercionKind funs axs tcs
-                                               (D & x ~ ki) (co ^ x)%Co _ in
-                       (TForAll ki (fst tys), TForAll ki (snd tys))
-    | CApp co1 co2 => let tys1 := coercionKind funs axs tcs D co1 _ in
-                      let tys2 := coercionKind funs axs tcs D co2 _ in
+    | CApp co1 co2 => let tys1 := coercionKind funs axs tcs co1 _ in
+                      let tys2 := coercionKind funs axs tcs co2 _ in
                       (TApp (fst tys1) (fst tys2), TApp (snd tys1) (snd tys2))
-    | CLeft co => let tys := coercionKind funs axs tcs D co _ in
+    | CLeft co => let tys := coercionKind funs axs tcs co _ in
                   match tys with
                     | (ty1, ty2) => _
                   end
-    | CRight co => let tys := coercionKind funs axs tcs D co _ in
+    | CRight co => let tys := coercionKind funs axs tcs co _ in
                    match tys with
                      | (ty1, ty2) => _
                    end
-    | CFun f co => let tys := coercionKind funs axs tcs D co _ in
+    | CFun f co => let tys := coercionKind funs axs tcs co _ in
                    (TFun f (fst tys), TFun f (snd tys))
     | CAx ax tys => match get ax axs with
                       | Some (mkAxiom kis f lhs rhs) => (TFun f (lhs[^tys]), rhs[^tys])
@@ -109,7 +128,7 @@ Obligation Tactic :=
   repeat abstract_sig;
   try omega;
   try solve [match goal with
-               | [ H : _;_ |-co _ ~: _ ~~ _ |- _ ] => inversion H
+               | [ H : _ |-co _ ~: _ ~~ _ |- _ ] => inversion H
              end; simpl; eauto].
 Hint Constructors co_kind.
 Solve Obligations.
@@ -121,47 +140,25 @@ Next Obligation.
   apply co_kind_det with (t1 := H) (t2 := t2) in H4; auto.
   apply co_kind_det with (t1 := t2) (t2 := H0) in H5; auto.
   intuition. subst. auto.
-Defined.
+Qed.
 
 Next Obligation.
   (* arrow result *)
   simpl. eauto.
-Defined.
-
-Next Obligation.
-  (* forall recursion *)
-  inversion H1.
-  remember (var_gen (dom D)) as x. specialize (H9 x). lapplies H9. eauto.
-  pose proof (@var_gen_spec (dom D)). eapply notin_subset. rewrite Heqx. apply H9.
-  admit. (* cofinite quantification *)
-Defined.
-
-Next Obligation.
-  (* forall size *)
-  unfold open_co. rewrite <- size_of_co_open. omega.
-Defined.
-
-Next Obligation.
-  (* forall result *)
-  simpl. inverts H1. econstructor. eassumption. simpl in H4.
-  pose proof H11.
-  specialize (H11 (var_gen (dom D))). lapplies H11.
-  apply co_kind_det with (t1 := t) (t2 := t0) in H0; auto. intuition. subst.
-  apply H. assumption. admit. (* cofinite quantification *)
-Defined.
+Qed.
 
 Next Obligation.
   simpl. eauto.
-Defined.
+Qed.
 
 Ltac cant_happen :=
   exfalso; inv_exists;
   match goal with
-    | [ H : _; _ |-co _ _ ~: _ ~~ _ |- _ ] => inverts H
+    | [ H : _ |-co _ _ ~: _ ~~ _ |- _ ] => inverts H
   end;
   match goal with
-    | [ H1 : _;_ |-co _ ~: TApp _ _ ~~ TApp _ _,
-        H2 : _;_ |-co _ ~: ?t3 ~~ ?t4 |- _ ] => apply co_kind_det with (t1 := t3) (t2 := t4) in H1; auto
+    | [ H1 : _ |-co _ ~: TApp _ _ ~~ TApp _ _,
+        H2 : _ |-co _ ~: ?t3 ~~ ?t4 |- _ ] => apply co_kind_det with (t1 := t3) (t2 := t4) in H1; auto
   end;
   intuition; discriminate.
 
@@ -174,7 +171,7 @@ Next Obligation.
   rewrite <- Heq_tys in *. simpls. clear Heqpair.
   destruct ty1; try cant_happen. destruct ty2; try cant_happen.
   apply (exist _ (ty1_1, ty2_1)). simpl. econstructor. eassumption.
-Defined.
+Qed.
 
 Next Obligation.
   (* right result *)
@@ -185,17 +182,17 @@ Next Obligation.
   rewrite <- Heq_tys in *. simpls. clear Heqpair.
   destruct ty1; try cant_happen. destruct ty2; try cant_happen.
   apply (exist _ (ty1_2, ty2_2)). simpl. econstructor. eassumption.
-Defined.
+Qed.
 
 Next Obligation.
   (* ax result *)
   inversion H1.
-  subst. econstructor; auto. pose proof H12 as Hcopy. apply binds_get in Hcopy.
+  subst. econstructor; auto. pose proof H10 as Hcopy. apply binds_get in Hcopy.
   rewrite Hcopy in Heq_anonymous. inverts Heq_anonymous. eassumption.
-Defined.
+Qed.
 
 Next Obligation.
   (* ax lookup failure impossible *)
-  exfalso. inv_exists. inverts H. apply binds_get in H10. rewrite H10 in Heq_anonymous.
+  exfalso. inv_exists. inverts H. apply binds_get in H8. rewrite H8 in Heq_anonymous.
   discriminate.
-Defined.
+Qed.
