coercion.v
@@ -1,107 +1,31 @@
 Require Import LibLN.
 Require Import List.
 
-Require Import type subst.
+Require Import type utils.
 
 Inductive coercion :=
 | CRefl : type -> coercion
 | CSym  : coercion -> coercion
 | CTrans : coercion -> coercion -> coercion
 | CArrow : coercion -> coercion -> coercion
-| CForAll : kind -> coercion -> coercion
 | CApp : coercion -> coercion -> coercion
 | CLeft : coercion -> coercion
 | CRight : coercion -> coercion
 | CFun : var -> coercion -> coercion
 | CAx : var -> list type -> coercion.
 
-Fixpoint open_co_rec (k : nat) (u : type) (co : coercion) {struct co} : coercion :=
+Inductive axiom :=
+| mkAxiom : list kind -> var -> type -> type -> axiom.
+
+Fixpoint size_of_co (fl : bool) co :=
   match co with
-    | CRefl ty => CRefl (open_rec k u ty)
-    | CSym co => CSym (open_co_rec k u co)
-    | CTrans co1 co2 => CTrans (open_co_rec k u co1) (open_co_rec k u co2)
-    | CArrow co1 co2 => CArrow (open_co_rec k u co1) (open_co_rec k u co2)
-    | CForAll ki co => CForAll ki (open_co_rec (S k) u co)
-    | CApp co1 co2 => CApp (open_co_rec k u co1) (open_co_rec k u co2)
-    | CLeft co => CLeft (open_co_rec k u co)
-    | CRight co => CRight (open_co_rec k u co)
-    | CFun f co => CFun f (open_co_rec k u co)
-    | CAx ax tys => CAx ax (map (open_rec k u) tys)
-  end.
-
-Definition open_co co u := open_co_rec 0 u co.
-
-Notation "{ k ~> u } t" := (open_co_rec k u t) (at level 66) : Co_scope.
-Notation "t ^^ u" := (open_co t u) (at level 67) : Co_scope.
-Notation "t ^ x" := (open_co t (TFVar (v x))) : Co_scope.
-
-Delimit Scope Co_scope with Co.
-Bind Scope Co_scope with coercion.
-
-Reserved Notation "Si ; D |-co g ~: t1 ~~ t2" (at level 67, t1 at next level).
-Inductive co_kind : gr_ctxt -> var_ctxt -> coercion -> type -> type -> Prop :=
-| CKRefl : forall Si D t k,
-             Si ; D |-ty t ~: k ->
-             (Si ; D |-co CRefl t ~: t ~~ t)
-| CKSym : forall Si D g t1 t2,
-            Si ; D |-co g ~: t1 ~~ t2 ->
-            Si ; D |-co CSym g ~: t2 ~~ t1
-| CKTrans : forall Si D g1 g2 t1 t2 t3,
-              Si ; D |-co g1 ~: t1 ~~ t2 ->
-              Si ; D |-co g2 ~: t2 ~~ t3 ->
-              Si ; D |-co CTrans g1 g2 ~: t1 ~~ t3
-| CKArrow : forall Si D g1 g2 t1 t1' t2 t2',
-              Si ; D |-co g1 ~: t1 ~~ t2 ->
-              Si ; D |-co g2 ~: t1' ~~ t2' ->
-              Si ; D |-co CArrow g1 g2 ~: TArrow t1 t1' ~~ TArrow t2 t2'
-| CKForAll : forall L Si D g k t1 t2,
-             dom D \c L ->
-             (forall a, a \notin L ->
-                        Si ; (D & a ~ k) |-co (g ^ a) ~: t1 ~~ t2) ->
-             Si ; D |-co CForAll k g ~: TForAll k t1 ~~ TForAll k t2
-| CKApp : forall Si D g1 g2 t1 t1' t2 t2',
-            Si ; D |-co g1 ~: t1 ~~ t2 ->
-            Si ; D |-co g2 ~: t1' ~~ t2' ->
-            Si ; D |-co CApp g1 g2 ~: TApp t1 t1' ~~ TApp t2 t2'
-| CKLeft : forall Si D g t1 t1' t2 t2',
-             Si ; D |-co g ~: TApp t1 t1' ~~ TApp t2 t2' ->
-             Si ; D |-co CLeft g ~: t1 ~~ t2
-| CKRight : forall Si D g t1 t1' t2 t2',
-              Si ; D |-co g ~: TApp t1 t1' ~~ TApp t2 t2' ->
-              Si ; D |-co CRight g ~: t1' ~~ t2'
-| CKFun : forall Si D g t1 t2 f,
-            Si ; D |-co g ~: t1 ~~ t2 ->
-            Si ; D |-co CFun f g ~: TFun f t1 ~~ TFun f t2
-| CKAx : forall ax ks f typat rhs axs funs tcs D tys,
-           ok_gr (funs, axs, tcs) -> ok D ->
-           binds ax (mkAxiom ks f typat rhs) axs ->
-           (funs, axs, tcs); D |-co CAx ax tys ~: TFun f (typat [^tys]) ~~ (rhs[^tys])
-where "Si ; D |-co g ~: t1 ~~ t2" := (co_kind Si D g t1 t2).
-
-Fixpoint sum ns :=
-  match ns with
-    | nil => 0
-    | x :: xs => x + sum xs
-  end.
-
-Lemma sum_app : forall xs ys,
-  sum (xs ++ ys) = sum xs + sum ys.
-Proof.
-  induction xs; intros.
-    simpl. auto.
-    simpl. rewrite IHxs. omega.
-Qed.
-
-Fixpoint size_of_co co :=
-  match co with
-    | CRefl ty => S (size_of_ty ty)
-    | CSym co => S (size_of_co co)
-    | CTrans co1 co2 => S (size_of_co co1 + size_of_co co2)
-    | CArrow co1 co2 => S (size_of_co co1 + size_of_co co2)
-    | CForAll k co => S (size_of_co co)
-    | CApp co1 co2 => S (size_of_co co1 + size_of_co co2)
-    | CLeft co => S (size_of_co co)
-    | CRight co => S (size_of_co co)
-    | CFun _ co => S (size_of_co co)
-    | CAx _ tys => S (sum (map size_of_ty tys))
+    | CRefl ty => S (size_of_ty fl ty)
+    | CSym co => S (size_of_co fl co)
+    | CTrans co1 co2 => S (size_of_co fl co1 + size_of_co fl co2)
+    | CArrow co1 co2 => S (size_of_co fl co1 + size_of_co fl co2)
+    | CApp co1 co2 => S (size_of_co fl co1 + size_of_co fl co2)
+    | CLeft co => S (size_of_co fl co)
+    | CRight co => S (size_of_co fl co)
+    | CFun _ co => S (size_of_co fl co)
+    | CAx _ tys => S (sum (map (size_of_ty fl) tys))
   end.
