compose.v
@@ -1,0 +1,10 @@
+Require Import Program.
+Require Import List.
+
+Lemma map_compose : forall A B C (f : B -> C) (g : A -> B) list,
+  map (f ∘ g) list = map f (map g list).
+Proof.
+  induction list.
+  - reflexivity.
+  - simpl. rewrite IHlist. unfold compose. reflexivity.
+Qed.
