ty_kind.v
@@ -1,0 +1,38 @@
+Require Import LibVar.
+Require Import LibEnv.
+
+Require Import type coercion.
+
+Set Implicit Variables.
+
+Definition fun_ctxt := env (kind * kind).
+Definition ax_ctxt  := env axiom.
+Definition tc_ctxt  := env kind.
+
+Definition ctxt := (fun_ctxt * ax_ctxt * tc_ctxt)%type.
+
+Definition ok_ctxt (Si : ctxt) :=
+  match Si with
+    | (funs, axs, tcs) => ok funs /\ ok axs /\ ok tcs
+  end.
+
+Reserved Notation "Si |-ty t ~: k" (at level 67).
+Inductive ty_kind : ctxt -> type -> kind -> Prop :=
+| TKFun : forall f k1 k2 funs axs tcs ty,
+            binds f (k1, k2) funs ->
+            (funs, axs, tcs) |-ty ty ~: k1 ->
+            (funs, axs, tcs) |-ty TFun f ty ~: k2
+| TKArrow : forall Si t1 t2,
+              Si |-ty t1 ~: KStar ->
+              Si |-ty t2 ~: KStar ->
+              Si |-ty TArrow t1 t2 ~: KStar
+| TKTyCon : forall tcs T k funs axs,
+              ok_ctxt (funs, axs, tcs) ->
+              binds T k tcs ->
+              (funs, axs, tcs) |-ty TTycon T ~: k
+| TKApp : forall Si t1 t2 k1 k2,
+            Si |-ty t1 ~: KArrow k1 k2 ->
+            Si |-ty t2 ~: k1 ->
+            Si |-ty TApp t1 t2 ~: k2
+where "Si |-ty t ~: k" := (ty_kind Si t k).
+
