var.v
@@ -1,0 +1,5 @@
+Require Import LibVar.
+
+Require Import utils.
+
+Axiom var_eq_decide : forall (v1 v2 : var), decide (v1 = v2).
